PR feedback

theories/CodegenWasm/LambdaANF_to_Wasm.v
@@ -406,24 +406,39 @@ Definition apply_binop_and_store_i64 (op : list basic_instruction) x y :=
   ] ++
   increment_global_mem_ptr 8.
 
-Definition make_carry (ord : nat) (gidx : N) : list basic_instruction :=
-    [ BI_global_get global_mem_ptr
-    ; BI_global_get gidx
-    ; BI_store T_i64 None 2%N 0%N
-    ; BI_global_get global_mem_ptr
-    ; BI_const_num (nat_to_value 8)
-    ; BI_binop T_i32 (Binop_i BOI_add)
-    ; BI_global_set constr_alloc_ptr
-    ; BI_global_get constr_alloc_ptr
-    ; BI_const_num (nat_to_value ord)
-    ; BI_store T_i32 None 2%N 0%N
-    ; BI_global_get global_mem_ptr
-    ; BI_const_num (nat_to_value 12)
-    ; BI_binop T_i32 (Binop_i BOI_add)
-    ; BI_global_get global_mem_ptr
-    ; BI_store T_i32 None 2%N 0%N
-    ; BI_global_get constr_alloc_ptr
+Definition make_carry (ord : nat) (gidx : globalidx) :=
+  [ BI_global_get global_mem_ptr
+  ; BI_global_get gidx
+  ; BI_store T_i64 None 2%N 0%N
+  ; BI_global_get global_mem_ptr
+  ; BI_const_num (nat_to_value 8)
+  ; BI_binop T_i32 (Binop_i BOI_add)
+  ; BI_global_set constr_alloc_ptr
+  ; BI_global_get constr_alloc_ptr
+  ; BI_const_num (nat_to_value ord)
+  ; BI_store T_i32 None 2%N 0%N
+  ; BI_global_get global_mem_ptr
+  ; BI_const_num (nat_to_value 12)
+  ; BI_binop T_i32 (Binop_i BOI_add)
+  ; BI_global_get global_mem_ptr
+  ; BI_store T_i32 None 2%N 0%N
+  ; BI_global_get constr_alloc_ptr
   ] ++ increment_global_mem_ptr 16.
+
+
+Definition apply_carry_operation x y  (ord1 ord2 : nat) (ops relops : list basic_instruction) : list basic_instruction :=
+    load_local_i64 x ++
+    load_local_i64 y ++
+    ops ++
+    [ BI_const_num maxuint63
+    ; BI_binop T_i64 (Binop_i BOI_and)
+    ; BI_global_set glob_tmp1
+    ] ++
+    relops ++
+    [ BI_if (BT_valtype (Some (T_num T_i32)))
+        (make_carry ord1 glob_tmp1)
+        (make_carry ord2 glob_tmp1)
+    ].
 
 (* Assumptions for constructing a prod value:
    - The 1st argument is stored in global gidx1, 2nd argument in global gidx2
@@ -461,6 +476,18 @@ Definition make_product (gidx1 gidx2 : N) : list basic_instruction :=
 
     ; BI_global_get constr_alloc_ptr
   ] ++ increment_global_mem_ptr 28.
+
+(* Assumptions about constructor environment for primitive operations that return bools:
+   1. ordinal(true) = 0
+   2. ordinal(false) = 1 *)
+Definition make_boolean_valued_comparison x y relop :=
+  load_local_i64 x ++            (* Load the arguments onto the stack *)
+  load_local_i64 y ++
+  [ BI_relop T_i64 (Relop_i relop)
+  ; BI_if (BT_valtype (Some (T_num T_i32)))
+      [ BI_const_num (nat_to_value 1) ] (* 2 * ordinal(true) + 1 *)
+      [ BI_const_num (nat_to_value 3) ] (* 2 * ordinal(false) + 1 *)
+  ].
 
 Definition translate_primitive_binary_op op_name x y : error (list basic_instruction) :=
   if Kername.eqb op_name primInt63Add then
@@ -521,41 +548,14 @@ Definition translate_primitive_binary_op op_name x y : error (list basic_instruc
          ; BI_global_get global_mem_ptr
          ] ++ increment_global_mem_ptr 8)
 
-  (* Assumptions about constructor environment for primitive operations that return bools:
-       1. ordinal(true) = 0
-       2. ordinal(false) = 1 *)
   else if Kername.eqb op_name primInt63Eqb then
-    Ret ([ BI_local_get x
-         ; BI_load T_i64 None 2%N 0%N
-         ; BI_local_get y
-         ; BI_load T_i64 None 2%N 0%N
-         ; BI_relop T_i64 (Relop_i ROI_eq)
-         ; BI_if (BT_valtype (Some (T_num T_i32)))
-             [ BI_const_num (nat_to_value 1) ] (* 2 * ordinal(true) + 1 *)
-             [ BI_const_num (nat_to_value 3) ] (* 2 * ordinal(false) + 1 *)
-         ])
+    Ret (make_boolean_valued_comparison x y ROI_eq)
 
   else if Kername.eqb op_name primInt63Ltb then
-    Ret ([ BI_local_get x
-         ; BI_load T_i64 None 2%N 0%N
-         ; BI_local_get y
-         ; BI_load T_i64 None 2%N 0%N
-         ; BI_relop T_i64 (Relop_i (ROI_lt SX_U))
-         ; BI_if (BT_valtype (Some (T_num T_i32)))
-             [ BI_const_num (nat_to_value 1) ] (* 2 * ordinal(true) + 1 *)
-             [ BI_const_num (nat_to_value 3) ] (* 2 * ordinal(false) + 1 *)
-         ])
+    Ret (make_boolean_valued_comparison x y (ROI_lt SX_U))
 
   else if Kername.eqb op_name primInt63Leb then
-    Ret ([ BI_local_get x
-         ; BI_load T_i64 None 2%N 0%N
-         ; BI_local_get y
-         ; BI_load T_i64 None 2%N 0%N
-         ; BI_relop T_i64 (Relop_i (ROI_le SX_U))
-         ; BI_if (BT_valtype (Some (T_num T_i32)))
-             [ BI_const_num (nat_to_value 1) ] (* 2 * ordinal(true) + 1 *)
-             [ BI_const_num (nat_to_value 3) ] (* 2 * ordinal(false) + 1 *)
-         ])
+    Ret (make_boolean_valued_comparison x y (ROI_le SX_U))
 
   (* Assumptions about constructor environment for compare:
        1. ordinal(Eq) = 0
@@ -583,72 +583,36 @@ Definition translate_primitive_binary_op op_name x y : error (list basic_instruc
           - ordinal(C0) = 0
           - ordinal(C1) = 1 *)
   else if Kername.eqb op_name primInt63Addc then
-    Ret(load_local_i64 x ++
-        load_local_i64 y ++
-        [ BI_binop T_i64 (Binop_i BOI_add)
-        ; BI_const_num maxuint63
-        ; BI_binop T_i64 (Binop_i BOI_and)
-        ; BI_global_set glob_tmp1
-        ; BI_global_get glob_tmp1
-        ] ++
-        load_local_i64 x ++
-        [ BI_relop T_i64 (Relop_i (ROI_lt SX_U))
-        ; BI_if (BT_valtype (Some (T_num T_i32)))
-            (make_carry 1 glob_tmp1)
-            (make_carry 0 glob_tmp1)
-        ])
+    Ret (apply_carry_operation x y 1 0
+           [ BI_binop T_i64 (Binop_i BOI_add) ]
+           ([ BI_global_get glob_tmp1 ] ++
+              load_local_i64 x ++
+              [ BI_relop T_i64 (Relop_i (ROI_lt SX_U))]))
 
   else if Kername.eqb op_name primInt63Addcarryc then
-    Ret(load_local_i64 x ++
-        load_local_i64 y ++
-        [ BI_binop T_i64 (Binop_i BOI_add)
-        ; BI_const_num (nat_to_value64 1)
-        ; BI_binop T_i64 (Binop_i BOI_add)
-        ; BI_const_num maxuint63
-        ; BI_binop T_i64 (Binop_i BOI_and)
-        ; BI_global_set glob_tmp1
-        ; BI_global_get glob_tmp1
-        ] ++
-        load_local_i64 x ++
-        [ BI_relop T_i64 (Relop_i (ROI_le SX_U))
-        ; BI_if (BT_valtype (Some (T_num T_i32)))
-            (make_carry 1 glob_tmp1)
-            (make_carry 0 glob_tmp1)
-        ])
+    Ret (apply_carry_operation x y 1 0
+           [ BI_binop T_i64 (Binop_i BOI_add)
+             ; BI_const_num (nat_to_value64 1)
+             ; BI_binop T_i64 (Binop_i BOI_add) ]
+           ([ BI_global_get glob_tmp1 ] ++
+              load_local_i64 x ++
+              [ BI_relop T_i64 (Relop_i (ROI_le SX_U))]))
 
   else if Kername.eqb op_name primInt63Subc then
-    Ret(load_local_i64 x ++
-        load_local_i64 y ++
-        [ BI_binop T_i64 (Binop_i BOI_sub)
-        ; BI_const_num maxuint63
-        ; BI_binop T_i64 (Binop_i BOI_and)
-        ; BI_global_set glob_tmp1
-        ] ++
-        load_local_i64 y ++
-        load_local_i64 x ++
-        [ BI_relop T_i64 (Relop_i (ROI_le SX_U))
-        ; BI_if (BT_valtype (Some (T_num T_i32)))
-            (make_carry 0 glob_tmp1)
-            (make_carry 1 glob_tmp1)
-        ])
+    Ret (apply_carry_operation x y 0 1
+           [ BI_binop T_i64 (Binop_i BOI_add) ]
+           (load_local_i64 y ++
+              load_local_i64 x ++
+              [ BI_relop T_i64 (Relop_i (ROI_le SX_U))]))
 
   else if Kername.eqb op_name primInt63Subcarryc then
-    Ret(load_local_i64 x ++
-        load_local_i64 y ++
-        [ BI_binop T_i64 (Binop_i BOI_sub)
-        ; BI_const_num (nat_to_value64 1)
-        ; BI_binop T_i64 (Binop_i BOI_sub)
-        ; BI_const_num maxuint63
-        ; BI_binop T_i64 (Binop_i BOI_and)
-        ; BI_global_set glob_tmp1
-        ] ++
-        load_local_i64 y ++
-        load_local_i64 x ++
-        [ BI_relop T_i64 (Relop_i (ROI_lt SX_U))
-        ; BI_if (BT_valtype (Some (T_num T_i32)))
-            (make_carry 0 glob_tmp1)
-            (make_carry 1 glob_tmp1)
-        ])
+    Ret (apply_carry_operation x y 0 1
+           [ BI_binop T_i64 (Binop_i BOI_add)
+           ; BI_const_num (nat_to_value64 1)
+           ; BI_binop T_i64 (Binop_i BOI_sub) ]
+           (load_local_i64 y ++
+              load_local_i64 x ++
+              [ BI_relop T_i64 (Relop_i (ROI_lt SX_U))]))
 
   else if Kername.eqb op_name primInt63Mulc then
     Ret (load_local_i64 x ++
